### CLRS Exercise 2.3-3: Exact Power of 2 Recurrence

**Problem Statement:**
Use mathematical induction to show that when $n$ is an exact power of 2, the solution to the recurrence
$$
T(n) = \begin{cases}
2 & \text{if } n = 2 \\
2T(n/2) + n & \text{if } n = 2^k, \text{ for } k > 1
\end{cases}
$$
is $T(n) = n \lg n$.

---

### Proof by Mathematical Induction

Let $n = 2^k$. We want to prove that $T(2^k) = 2^k \lg(2^k) = k \cdot 2^k$.

#### 1. Base Case
For $k=1$, we have $n = 2^1 = 2$.
* **From the Formula:** $n \lg n = 2 \lg 2 = 2(1) = 2$.
* **From the Recurrence:** $T(2) = 2$.
Since $2 = 2$, the base case holds.

#### 2. Inductive Hypothesis
Assume that for some arbitrary integer $k > 1$, the formula holds:
$$
T(2^k) = k \cdot 2^k
$$

#### 3. Inductive Step
We must prove that the formula holds for $k+1$. That is, we must show that $T(2^{k+1}) = (k+1) 2^{k+1}$.

Using the recurrence definition for $n = 2^{k+1}$:
$$
T(2^{k+1}) = 2T\left( \frac{2^{k+1}}{2} \right) + 2^{k+1}
$$
Simplify the fraction inside $T(\cdot)$:
$$
T(2^{k+1}) = 2T(2^k) + 2^{k+1}
$$
Substitute the **Inductive Hypothesis** ($T(2^k) = k \cdot 2^k$):
$$
\begin{align}
T(2^{k+1}) &= 2(k \cdot 2^k) + 2^{k+1} \\
&= k \cdot 2^{k+1} + 2^{k+1}
\end{align}
$$
Factor out $2^{k+1}$:
$$
\begin{align}
T(2^{k+1}) &= 2^{k+1} (k + 1) \\
&= (k+1) 2^{k+1}
\end{align}
$$

#### Conclusion
By the principle of mathematical induction, $T(n) = n \lg n$ for all $n$ that are exact powers of 2.
